rocq/theories/TypeSystem/CheckerUsageSoundness.v
@@ -102,6 +102,7 @@ Fixpoint expr_linear_lets_used (fenv : list fn_def) (e : expr) {struct e}
   | EUnit => True
   | ELit _ => True
   | EVar _ => True
+  | EFn _ => True
   | ELet m x T e1 e2 =>
       (ty_usage T = ULinear ->
        forall Ω n Γ Γout T2,
@@ -116,6 +117,7 @@ Fixpoint expr_linear_lets_used (fenv : list fn_def) (e : expr) {struct e}
       expr_linear_lets_used fenv e1 /\
       expr_linear_lets_used fenv e2
   | ECall _ _ => True
+  | ECallExpr _ _ => True
   | EReplace _ e_new => expr_linear_lets_used fenv e_new
   | EAssign _ e_new => expr_linear_lets_used fenv e_new
   | EBorrow _ _ => True
